\begin{report}
    This is a proof by induction on the form of the assumed sequent
    $ \FILLnt{A_{{\mathrm{1}}}}  \FILLsym{,} \, ... \, \FILLsym{,}  \FILLnt{A_{\FILLmv{i}}}  \vdash  \FILLnt{B_{{\mathrm{1}}}}  \FILLsym{,} \, ... \, \FILLsym{,}  \FILLnt{B_{\FILLmv{j}}} $.  Throughout the proof if $\Gamma =
    \FILLnt{A_{{\mathrm{1}}}}  \FILLsym{,} \, ... \, \FILLsym{,}  \FILLnt{A_{\FILLmv{i}}}$, then $ \lnot (  ( \Gamma )^N  )  = \FILLmv{x_{{\mathrm{1}}}}  \FILLsym{:}   \lnot  \FILLsym{(}   ( \FILLnt{A_{{\mathrm{1}}}} )^N   \FILLsym{)}   \FILLsym{,} \, ... \, \FILLsym{,}  \FILLmv{x_{\FILLmv{i}}}  \FILLsym{:}   \lnot  \FILLsym{(}   ( \FILLnt{A_{\FILLmv{i}}} )^N   \FILLsym{)} $ for some unique fresh variables
    $\FILLmv{x_{{\mathrm{1}}}},\ldots,\FILLmv{x_{\FILLmv{i}}}$.  We will use this notation when applying
    the inductive hypothesis to make the presentation easier to read.
  \begin{itemize}
  \item[] Case.\\ 
    \begin{center}
      \begin{math}
        $$\mprset{flushleft}
        \inferrule* [right=\ifrName{Ax}] {
          \ 
        }{ \FILLnt{A}  \vdash  \FILLnt{A} }
      \end{math}
    \end{center}
    It suffices to derive the sequent
    $ \FILLmv{x}  \FILLsym{:}   \lnot    \lnot  \FILLsym{(}   ( \FILLnt{A} )^N   \FILLsym{)}     \FILLsym{,}  \FILLmv{y}  \FILLsym{:}   \lnot  \FILLsym{(}   ( \FILLnt{A} )^N   \FILLsym{)}   \vdash   \cdot  $
    which is equivalent to the sequent
    $ \FILLmv{x}  \FILLsym{:}     \lnot  \FILLsym{(}   ( \FILLnt{A} )^N   \FILLsym{)}    \multimap    \perp    \FILLsym{,}  \FILLmv{y}  \FILLsym{:}   \lnot  \FILLsym{(}   ( \FILLnt{A} )^N   \FILLsym{)}   \vdash   \cdot  $.  The latter is
    derivable as follows:
    \begin{center}
      \begin{math}
        $$\mprset{flushleft}
        \inferrule* [right=Impl] {
          $$\mprset{flushleft}
          \inferrule* [right=Ax] {
            \,
          }{ \FILLmv{y}  \FILLsym{:}   \lnot  \FILLsym{(}   ( \FILLnt{A} )^N   \FILLsym{)}   \vdash  \FILLmv{y}  \FILLsym{:}   \lnot  \FILLsym{(}   ( \FILLnt{A} )^N   \FILLsym{)}  }
          \\
          $$\mprset{flushleft}
          \inferrule* [right=Pl] {
            \,
          }{ \FILLmv{w}  \FILLsym{:}   \perp   \vdash   \cdot  }
        }{ \FILLmv{x}  \FILLsym{:}     \lnot  \FILLsym{(}   ( \FILLnt{A} )^N   \FILLsym{)}    \multimap    \perp    \FILLsym{,}  \FILLmv{y}  \FILLsym{:}   \lnot  \FILLsym{(}   ( \FILLnt{A} )^N   \FILLsym{)}   \vdash   \cdot  }
      \end{math}
    \end{center}
    

  \item[] Case.\\ 
    \begin{center}
      \begin{math}
        $$\mprset{flushleft}
        \inferrule* [right=\ifrName{Cut}] {
            \Gamma_{{\mathrm{1}}}  \vdash  \FILLnt{A}  \FILLsym{,}  \Delta_{{\mathrm{1}}}   \quad   \Gamma_{{\mathrm{2}}}  \FILLsym{,}  \FILLnt{A}  \vdash  \Delta_{{\mathrm{2}}}  
        }{ \Gamma_{{\mathrm{1}}}  \FILLsym{,}  \Gamma_{{\mathrm{2}}}  \vdash  \Delta_{{\mathrm{1}}}  \FILLsym{,}  \Delta_{{\mathrm{2}}} }
      \end{math}
    \end{center}
    By the induction hypothesis we know the following:
    \begin{center}
      \begin{math}
        \begin{array}{lll}
            \lnot (  \lnot (  ( \Gamma_{{\mathrm{1}}} )^N  )  )   \FILLsym{,}  \FILLmv{x}  \FILLsym{:}   \lnot  \FILLsym{(}   ( \FILLnt{A} )^N   \FILLsym{)}   \FILLsym{,}   \lnot (  ( \Delta_{{\mathrm{1}}} )^N  )   \vdash   \cdot  \\
            \lnot (  \lnot (  ( \Gamma_{{\mathrm{2}}} )^N  )  )   \FILLsym{,}  \FILLmv{y}  \FILLsym{:}   \lnot  \FILLsym{(}   \lnot  \FILLsym{(}   ( \FILLnt{A} )^N   \FILLsym{)}   \FILLsym{)}   \FILLsym{,}   \lnot (  ( \Delta_{{\mathrm{2}}} )^N  )   \vdash   \cdot  
        \end{array}
      \end{math}
    \end{center}
    It suffices to derive the sequent $  \lnot (  \lnot (  ( \Gamma_{{\mathrm{1}}} )^N  )  )   \FILLsym{,}   \lnot (  \lnot (  ( \Gamma_{{\mathrm{2}}} )^N  )  )   \FILLsym{,}   \lnot (  ( \Delta_{{\mathrm{1}}} )^N  )   \FILLsym{,}   \lnot (  ( \Delta_{{\mathrm{2}}} )^N  )   \vdash   \cdot  $ which we do as follows:
    \begin{center}
      \begin{math}
        $$\mprset{flushleft}
        \inferrule* [right=Cut] {
          $$\mprset{flushleft}
        \inferrule* [right=Impr] {
          $$\mprset{flushleft}
        \inferrule* [right=Pr] {
            \lnot (  \lnot (  ( \Gamma_{{\mathrm{1}}} )^N  )  )   \FILLsym{,}  \FILLmv{x}  \FILLsym{:}   \lnot  \FILLsym{(}   ( \FILLnt{A} )^N   \FILLsym{)}   \FILLsym{,}   \lnot (  ( \Delta_{{\mathrm{1}}} )^N  )   \vdash   \cdot  
        }{  \lnot (  \lnot (  ( \Gamma_{{\mathrm{1}}} )^N  )  )   \FILLsym{,}  \FILLmv{x}  \FILLsym{:}   \lnot  \FILLsym{(}   ( \FILLnt{A} )^N   \FILLsym{)}   \FILLsym{,}   \lnot (  ( \Delta_{{\mathrm{1}}} )^N  )   \vdash   \circ   \FILLsym{:}   \perp  }
        }{  \lnot (  \lnot (  ( \Gamma_{{\mathrm{1}}} )^N  )  )   \FILLsym{,}   \lnot (  ( \Delta_{{\mathrm{1}}} )^N  )   \vdash   \lambda  \FILLmv{x}  .   \circ    \FILLsym{:}   \lnot  \FILLsym{(}   \lnot  \FILLsym{(}   ( \FILLnt{A} )^N   \FILLsym{)}   \FILLsym{)}  }
        \\
          \lnot (  \lnot (  ( \Gamma_{{\mathrm{2}}} )^N  )  )   \FILLsym{,}  \FILLmv{y}  \FILLsym{:}   \lnot  \FILLsym{(}   \lnot  \FILLsym{(}   ( \FILLnt{A} )^N   \FILLsym{)}   \FILLsym{)}   \FILLsym{,}   \lnot (  ( \Delta_{{\mathrm{2}}} )^N  )   \vdash   \cdot  
        }{  \lnot (  \lnot (  ( \Gamma_{{\mathrm{1}}} )^N  )  )   \FILLsym{,}   \lnot (  \lnot (  ( \Gamma_{{\mathrm{2}}} )^N  )  )   \FILLsym{,}   \lnot (  ( \Delta_{{\mathrm{1}}} )^N  )   \FILLsym{,}   \lnot (  ( \Delta_{{\mathrm{2}}} )^N  )   \vdash   \cdot  }
      \end{math}
    \end{center}

  \item[] Case.\\ 
    \begin{center}
      \begin{math}
        $$\mprset{flushleft}
        \inferrule* [right=\ifrName{Tl}] {
           \Gamma  \vdash  \Delta 
        }{ \Gamma  \FILLsym{,}   \top   \vdash  \Delta }
      \end{math}
    \end{center}
    First, note that $ (  \top  )^N  =  \top $.  By the induction hypothesis
    we know $  \lnot (  \lnot (  ( \Gamma )^N  )  )   \FILLsym{,}   \lnot (  ( \Delta )^N  )   \vdash   \cdot  $.  We obtain our result by
    the following derivation:
    \begin{center}
      \begin{math}
        $$\mprset{flushleft}
        \inferrule* [right=Impl] {
          $$\mprset{flushleft}
          \inferrule* [right=Impr] {
            $$\mprset{flushleft}
            \inferrule* [right=Pr] {
              $$\mprset{flushleft}
              \inferrule* [right=Tl] {
                  \lnot (  \lnot (  ( \Gamma )^N  )  )   \FILLsym{,}   \lnot (  ( \Delta )^N  )   \vdash   \cdot  
              }{  \lnot (  \lnot (  ( \Gamma )^N  )  )   \FILLsym{,}   \lnot (  ( \Delta )^N  )   \FILLsym{,}  \FILLmv{z}  \FILLsym{:}   \top   \vdash   \cdot  }
            }{  \lnot (  \lnot (  ( \Gamma )^N  )  )   \FILLsym{,}   \lnot (  ( \Delta )^N  )   \FILLsym{,}  \FILLmv{z}  \FILLsym{:}   \top   \vdash  \FILLnt{t}  \FILLsym{:}   \perp  }
          }{  \lnot (  \lnot (  ( \Gamma )^N  )  )   \FILLsym{,}   \lnot (  ( \Delta )^N  )   \vdash  \FILLnt{t}  \FILLsym{:}   \lnot   \top   }
          \\
          $$\mprset{flushleft}
          \inferrule* [right=Pl] {
            \,
          }{ \FILLmv{y}  \FILLsym{:}   \perp   \vdash   \cdot  }
        }{  \lnot (  \lnot (  ( \Gamma )^N  )  )   \FILLsym{,}  \FILLmv{x}  \FILLsym{:}   \lnot  \FILLsym{(}   \lnot   \top    \FILLsym{)}   \FILLsym{,}   \lnot (  ( \Delta )^N  )   \vdash   \cdot  }
      \end{math}
    \end{center}
    Note that $ \mathsf{let}\, \FILLmv{x} \,\mathsf{be}\,  *  \,\mathsf{in}\,  \cdot   = \cdot$ for any variable $\FILLmv{x}$.

  \item[] Case.\\ 
    \begin{center}
      \begin{math}
        $$\mprset{flushleft}
        \inferrule* [right=\ifrName{Tr}] {
          \ 
        }{  \cdot   \vdash   \top  }
      \end{math}
    \end{center}
    If suffices to derive the sequent $ \FILLmv{x}  \FILLsym{:}   \lnot  \FILLsym{(}   (  \top  )^N   \FILLsym{)}   \vdash   \cdot  $, but this is equivalent to the sequent
    $ \FILLmv{x}  \FILLsym{:}   \lnot   \top    \vdash   \cdot  $ which is derivable as follows:
    \begin{center}
      \begin{math}
        $$\mprset{flushleft}
        \inferrule* [right=Impl] {
          $$\mprset{flushleft}
          \inferrule* [right=Tr] {
            \,
          }{  \cdot   \vdash  \FILLsym{*}  \FILLsym{:}   \top  }
          \\
            $$\mprset{flushleft}
          \inferrule* [right=Pl] {
            \,
          }{ \FILLmv{y}  \FILLsym{:}   \perp   \vdash   \cdot  }
        }{ \FILLmv{x}  \FILLsym{:}   \lnot   \top    \vdash   \cdot  }
      \end{math}
    \end{center}
    
  \item[] Case.\\ 
    \begin{center}
      \begin{math}
        $$\mprset{flushleft}
        \inferrule* [right=\ifrName{Tenl}] {
           \Gamma  \FILLsym{,}  \FILLnt{A}  \FILLsym{,}  \FILLnt{B}  \vdash  \Delta 
        }{ \Gamma  \FILLsym{,}   \FILLnt{A}  \otimes  \FILLnt{B}   \vdash  \Delta }
      \end{math}
    \end{center}
    By the induction hypothesis we have the following sequent:
    \begin{center}
      \begin{math}
        \begin{array}{lll}
            \lnot (  \lnot (  ( \Gamma )^N  )  )   \FILLsym{,}  \FILLmv{x}  \FILLsym{:}   \lnot    \lnot  \FILLsym{(}   ( \FILLnt{A} )^N   \FILLsym{)}     \FILLsym{,}  \FILLmv{y}  \FILLsym{:}   \lnot    \lnot  \FILLsym{(}   ( \FILLnt{B} )^N   \FILLsym{)}     \FILLsym{,}   \lnot (  ( \Delta )^N  )   \vdash   \cdot  
        \end{array}
      \end{math}
    \end{center}
    Our result follows from the following derivation:
    \begin{center}
      \begin{math}
        $$\mprset{flushleft}
        \inferrule* [right=Impl] {
         $$\mprset{flushleft}
          \inferrule* [right=Impr] {
            $$\mprset{flushleft}
            \inferrule* [right=Tenl] {
              $$\mprset{flushleft}
              \inferrule* [right=Pr] {
                  \lnot (  \lnot (  ( \Gamma )^N  )  )   \FILLsym{,}  \FILLmv{w}  \FILLsym{:}    \lnot    \lnot  \FILLsym{(}   ( \FILLnt{A} )^N   \FILLsym{)}      \FILLsym{,}  \FILLmv{v}  \FILLsym{:}   \lnot    \lnot  \FILLsym{(}   ( \FILLnt{B} )^N   \FILLsym{)}     \FILLsym{,}   \lnot (  ( \Delta )^N  )   \vdash   \cdot  
              }{  \lnot (  \lnot (  ( \Gamma )^N  )  )   \FILLsym{,}  \FILLmv{w}  \FILLsym{:}    \lnot    \lnot  \FILLsym{(}   ( \FILLnt{A} )^N   \FILLsym{)}      \FILLsym{,}  \FILLmv{v}  \FILLsym{:}   \lnot    \lnot  \FILLsym{(}   ( \FILLnt{B} )^N   \FILLsym{)}     \FILLsym{,}   \lnot (  ( \Delta )^N  )   \vdash   \circ   \FILLsym{:}   \perp  }
            }{  \lnot (  \lnot (  ( \Gamma )^N  )  )   \FILLsym{,}  \FILLmv{x}  \FILLsym{:}     \lnot    \lnot  \FILLsym{(}   ( \FILLnt{A} )^N   \FILLsym{)}      \otimes   \lnot    \lnot  \FILLsym{(}   ( \FILLnt{B} )^N   \FILLsym{)}      \FILLsym{,}   \lnot (  ( \Delta )^N  )   \vdash    \mathsf{let}\, \FILLmv{x} \,\mathsf{be}\, \FILLsym{(}   \FILLmv{w}  \otimes  \FILLmv{v}   \FILLsym{)} \,\mathsf{in}\,  \circ     \FILLsym{:}   \perp  }
          }{   \lnot (  \lnot (  ( \Gamma )^N  )  )   \FILLsym{,}   \lnot (  ( \Delta )^N  )   \vdash   \lambda  \FILLmv{x}  .    \mathsf{let}\, \FILLmv{x} \,\mathsf{be}\, \FILLsym{(}   \FILLmv{w}  \otimes  \FILLmv{v}   \FILLsym{)} \,\mathsf{in}\,  \circ      \FILLsym{:}   \lnot  \FILLsym{(}     \lnot    \lnot  \FILLsym{(}   ( \FILLnt{A} )^N   \FILLsym{)}      \otimes   \lnot    \lnot  \FILLsym{(}   ( \FILLnt{B} )^N   \FILLsym{)}      \FILLsym{)}  }
          \\
          $$\mprset{flushleft}
          \inferrule* [right=Pl] {
            \,
          }{ \FILLmv{y}  \FILLsym{:}   \perp   \vdash   \cdot  }
        }{  \lnot (  \lnot (  ( \Gamma )^N  )  )   \FILLsym{,}  \FILLmv{z}  \FILLsym{:}   \lnot    \lnot  \FILLsym{(}     \lnot    \lnot  \FILLsym{(}   ( \FILLnt{A} )^N   \FILLsym{)}      \otimes   \lnot    \lnot  \FILLsym{(}   ( \FILLnt{B} )^N   \FILLsym{)}      \FILLsym{)}     \FILLsym{,}   \lnot (  ( \Delta )^N  )   \vdash   \cdot  }
      \end{math}
    \end{center}

  \item[] Case.\\ 
    \begin{center}
      \begin{math}
        $$\mprset{flushleft}
        \inferrule* [right=\ifrName{Tenr}] {
            \Gamma  \vdash  \FILLnt{A}  \FILLsym{,}  \Delta   \quad   \Gamma'  \vdash  \FILLnt{B}  \FILLsym{,}  \Delta'  
        }{ \Gamma  \FILLsym{,}  \Gamma'  \vdash     \FILLnt{A}  \otimes  \FILLnt{B}    \FILLsym{,}  \Delta   \FILLsym{,}  \Delta' }
      \end{math}
    \end{center}
    By the induction hypothesis we know the following:
    \begin{center}
      \begin{math}
        \begin{array}{lll}
            \lnot (  \lnot (  ( \Gamma )^N  )  )   \FILLsym{,}  \FILLmv{x}  \FILLsym{:}    \lnot  \FILLsym{(}   ( \FILLnt{A} )^N   \FILLsym{)}    \FILLsym{,}   \lnot (  ( \Delta )^N  )   \vdash   \cdot  \\
            \lnot (  \lnot (  ( \Gamma' )^N  )  )   \FILLsym{,}  \FILLmv{y}  \FILLsym{:}    \lnot  \FILLsym{(}   ( \FILLnt{B} )^N   \FILLsym{)}    \FILLsym{,}   \lnot (  ( \Delta' )^N  )   \vdash   \cdot  \\
        \end{array}
      \end{math}
    \end{center}
    We obtain our result by the following derivation:
    \begin{center}
      \tiny
      \begin{math}
        $$\mprset{flushleft}
        \inferrule* [right=\ifrName{Impl}] {
          $$\mprset{flushleft}
          \inferrule* [right=\ifrName{Tenr}] {
            $$\mprset{flushleft}
            \inferrule* [right=\ifrName{Impr}] {
              $$\mprset{flushleft}
              \inferrule* [right=\ifrName{Pr}] {
                  \lnot (  \lnot (  ( \Gamma )^N  )  )   \FILLsym{,}  \FILLmv{x}  \FILLsym{:}   \lnot  \FILLsym{(}   ( \FILLnt{A} )^N   \FILLsym{)}   \FILLsym{,}   \lnot (  ( \Delta )^N  )   \vdash   \cdot  
              }{  \lnot (  \lnot (  ( \Gamma )^N  )  )   \FILLsym{,}  \FILLmv{x}  \FILLsym{:}   \lnot  \FILLsym{(}   ( \FILLnt{A} )^N   \FILLsym{)}   \FILLsym{,}   \lnot (  ( \Delta )^N  )   \vdash   \circ   \FILLsym{:}   \perp  }
            }{  \lnot (  \lnot (  ( \Gamma )^N  )  )   \FILLsym{,}   \lnot (  ( \Delta )^N  )   \vdash   \lambda  \FILLmv{x}  .   \circ    \FILLsym{:}    \lnot    \lnot  \FILLsym{(}   ( \FILLnt{A} )^N   \FILLsym{)}     }
            \\
            $$\mprset{flushleft}
            \inferrule* [right=\ifrName{Impr}] {
              $$\mprset{flushleft}
              \inferrule* [right=\ifrName{Pr}] {
                  \lnot (  \lnot (  ( \Gamma' )^N  )  )   \FILLsym{,}  \FILLmv{y}  \FILLsym{:}   \lnot  \FILLsym{(}   ( \FILLnt{B} )^N   \FILLsym{)}   \FILLsym{,}   \lnot (  ( \Delta' )^N  )   \vdash   \cdot  
              }{  \lnot (  \lnot (  ( \Gamma' )^N  )  )   \FILLsym{,}  \FILLmv{y}  \FILLsym{:}   \lnot  \FILLsym{(}   ( \FILLnt{B} )^N   \FILLsym{)}   \FILLsym{,}   \lnot (  ( \Delta' )^N  )   \vdash   \circ   \FILLsym{:}   \perp  }
            }{  \lnot (  \lnot (  ( \Gamma' )^N  )  )   \FILLsym{,}   \lnot (  ( \Delta' )^N  )   \vdash   \lambda  \FILLmv{y}  .   \circ    \FILLsym{:}   \lnot    \lnot  \FILLsym{(}   ( \FILLnt{B} )^N   \FILLsym{)}    }
          }{  \lnot (  \lnot (  ( \Gamma )^N  )  )   \FILLsym{,}   \lnot (  \lnot (  ( \Gamma' )^N  )  )   \FILLsym{,}   \lnot (  ( \Delta )^N  )   \FILLsym{,}   \lnot (  ( \Delta' )^N  )   \vdash    (  \lambda  \FILLmv{x}  .   \circ   )   \otimes   (  \lambda  \FILLmv{y}  .   \circ   )    \FILLsym{:}     \lnot    \lnot  \FILLsym{(}   ( \FILLnt{A} )^N   \FILLsym{)}      \otimes   \lnot    \lnot  \FILLsym{(}   ( \FILLnt{B} )^N   \FILLsym{)}     }
          \\
          $$\mprset{flushleft}
          \inferrule* [right=\ifrName{Pl}] {
            \,
          }{ \FILLmv{w}  \FILLsym{:}   \perp   \vdash   \cdot  }
        }{  \lnot (  \lnot (  ( \Gamma )^N  )  )   \FILLsym{,}   \lnot (  \lnot (  ( \Gamma' )^N  )  )   \FILLsym{,}  \FILLmv{z}  \FILLsym{:}    \lnot  \FILLsym{(}     \lnot    \lnot  \FILLsym{(}   ( \FILLnt{A} )^N   \FILLsym{)}      \otimes   \lnot    \lnot  \FILLsym{(}   ( \FILLnt{B} )^N   \FILLsym{)}      \FILLsym{)}    \FILLsym{,}   \lnot (  ( \Delta )^N  )   \FILLsym{,}   \lnot (  ( \Delta' )^N  )   \vdash   \cdot  }
      \end{math}
    \end{center}

  \item[] Case.\\ 
    \begin{center}
      \begin{math}
        $$\mprset{flushleft}
        \inferrule* [right=\ifrName{Pl}] {
          \ 
        }{  \perp   \vdash   \cdot  }
      \end{math}
    \end{center}
    It suffices to show that $ \FILLmv{z}  \FILLsym{:}   \lnot  \FILLsym{(}   (  \perp  )^N   \FILLsym{)}   \vdash   \cdot  $ is derivable, which is equivalent to showing that
    the sequent $ \FILLmv{z}  \FILLsym{:}   \lnot    \lnot  \FILLsym{(}   \perp   \FILLsym{)}     \vdash   \cdot  $ is derivable.  We obtain our result by the following derivation:
    \begin{center}
      \begin{math}
        $$\mprset{flushleft}
        \inferrule* [right=Impl] {
          $$\mprset{flushleft}
          \inferrule* [right=Impr] {
            $$\mprset{flushleft}
            \inferrule* [right=Pr] {
              $$\mprset{flushleft}
              \inferrule* [right=Pl] {
                \,
              }{ \FILLmv{x}  \FILLsym{:}   \perp   \vdash   \cdot  }
            }{ \FILLmv{x}  \FILLsym{:}   \perp   \vdash   \circ   \FILLsym{:}   \perp  }
          }{  \cdot   \vdash   \lambda  \FILLmv{x}  .   \circ    \FILLsym{:}   \lnot  \FILLsym{(}   \perp   \FILLsym{)}  }
          \\
            $$\mprset{flushleft}
          \inferrule* [right=Pl] {
            \,
          }{ \FILLmv{w}  \FILLsym{:}   \perp   \vdash   \cdot  }
        }{ \FILLmv{z}  \FILLsym{:}   \lnot    \lnot  \FILLsym{(}   \perp   \FILLsym{)}     \vdash   \cdot  }
      \end{math}
    \end{center}


  \item[] Case.\\ 
    \begin{center}
      \begin{math}
        $$\mprset{flushleft}
        \inferrule* [right=\ifrName{Pr}] {
           \Gamma  \vdash  \Delta 
        }{ \Gamma  \vdash   \perp   \FILLsym{,}  \Delta }
      \end{math}
    \end{center}
    By the induction hypothesis we know the following sequent is derivable:
    \[
        \lnot (  \lnot (  ( \Gamma )^N  )  )   \FILLsym{,}   \lnot (  ( \Delta )^N  )   \vdash   \cdot  
    \]
    It suffices to show that $  \lnot (  \lnot (  ( \Gamma )^N  )  )   \FILLsym{,}  \FILLmv{z}  \FILLsym{:}   \lnot  \FILLsym{(}   (  \perp  )^N   \FILLsym{)}   \FILLsym{,}   \lnot (  ( \Delta )^N  )   \vdash   \cdot  $ which is equivalent to
    the sequent $  \lnot (  \lnot (  ( \Gamma )^N  )  )   \FILLsym{,}  \FILLmv{z}  \FILLsym{:}   \lnot  \FILLsym{(}   \perp   \FILLsym{)}   \FILLsym{,}   \lnot (  ( \Delta )^N  )   \vdash   \cdot  $.  The latter is derivable as follows:
    \begin{center}
      \begin{math}
        $$\mprset{flushleft}
        \inferrule* [right=Impl] {
          $$\mprset{flushleft}
          \inferrule* [right=Pr] {
              \lnot (  \lnot (  ( \Gamma )^N  )  )   \FILLsym{,}   \lnot (  ( \Delta )^N  )   \vdash   \cdot  
          }{  \lnot (  \lnot (  ( \Gamma )^N  )  )   \FILLsym{,}   \lnot (  ( \Delta )^N  )   \vdash   \circ   \FILLsym{:}   \perp  }
          \\
            $$\mprset{flushleft}
          \inferrule* [right=Pl] {
            \,
          }{ \FILLmv{w}  \FILLsym{:}   \perp   \vdash   \cdot  }
        }{  \lnot (  \lnot (  ( \Gamma )^N  )  )   \FILLsym{,}  \FILLmv{z}  \FILLsym{:}   \lnot  \FILLsym{(}   \perp   \FILLsym{)}   \FILLsym{,}   \lnot (  ( \Delta )^N  )   \vdash   \cdot  }
      \end{math}
    \end{center}
    
  \item[] Case.\\ 
    \begin{center}
      \begin{math}
        $$\mprset{flushleft}
        \inferrule* [right=\ifrName{Parl}] {
            \Gamma  \FILLsym{,}  \FILLnt{A}  \vdash  \Delta   \quad   \Gamma'  \FILLsym{,}  \FILLnt{B}  \vdash  \Delta'  
        }{ \Gamma  \FILLsym{,}  \Gamma'  \FILLsym{,}   \FILLnt{A}  \parr  \FILLnt{B}   \vdash  \Delta  \FILLsym{,}  \Delta' }
      \end{math}
    \end{center}
    By the induction hypothesis we know the following:
    \begin{center}
      \begin{math}
        \begin{array}{lll}
            \lnot (  \lnot (  ( \Gamma )^N  )  )   \FILLsym{,}  \FILLmv{x}  \FILLsym{:}   \lnot    \lnot  \FILLsym{(}   ( \FILLnt{A} )^N   \FILLsym{)}     \FILLsym{,}   \lnot (  ( \Delta )^N  )   \vdash   \cdot  \\
            \lnot (  \lnot (  ( \Gamma' )^N  )  )   \FILLsym{,}  \FILLmv{v}  \FILLsym{:}   \lnot    \lnot  \FILLsym{(}   ( \FILLnt{B} )^N   \FILLsym{)}     \FILLsym{,}   \lnot (  ( \Delta' )^N  )   \vdash   \cdot  
        \end{array}
      \end{math}
    \end{center}
    It suffices to show that the sequent
    \[   \lnot (  \lnot (  ( \Gamma )^N  )  )   \FILLsym{,}   \lnot (  \lnot (  ( \Gamma' )^N  )  )   \FILLsym{,}  \FILLmv{z}  \FILLsym{:}   \lnot    \lnot  \FILLsym{(}   (  \FILLnt{A}  \parr  \FILLnt{B}  )^N   \FILLsym{)}     \FILLsym{,}   \lnot (  ( \Delta )^N  )   \FILLsym{,}   \lnot (  ( \Delta' )^N  )   \vdash   \cdot   \]
    is derivable which is equivalent to the sequent
    \[   \lnot (  \lnot (  ( \Gamma )^N  )  )   \FILLsym{,}   \lnot (  \lnot (  ( \Gamma' )^N  )  )   \FILLsym{,}  \FILLmv{z}  \FILLsym{:}   \lnot    \lnot  \FILLsym{(}     \lnot    \lnot  \FILLsym{(}   ( \FILLnt{A} )^N   \FILLsym{)}      \parr   \lnot    \lnot  \FILLsym{(}   ( \FILLnt{B} )^N   \FILLsym{)}      \FILLsym{)}     \FILLsym{,}   \lnot (  ( \Delta )^N  )   \FILLsym{,}   \lnot (  ( \Delta' )^N  )   \vdash   \cdot  . \]
    The latter is derivable as follows:
    \begin{center}
      \begin{math}        
        $$\mprset{flushleft}
        \inferrule* [right=\ifrName{Impl}] {
          D
          \\
            $$\mprset{flushleft}
          \inferrule* [right=\ifrName{Pl}] {
            \,
          }{ \FILLmv{w}  \FILLsym{:}   \perp   \vdash   \cdot  }
        }{  \lnot (  \lnot (  ( \Gamma )^N  )  )   \FILLsym{,}   \lnot (  \lnot (  ( \Gamma' )^N  )  )   \FILLsym{,}  \FILLmv{z}  \FILLsym{:}   \lnot    \lnot  \FILLsym{(}     \lnot    \lnot  \FILLsym{(}   ( \FILLnt{A} )^N   \FILLsym{)}      \parr   \lnot    \lnot  \FILLsym{(}   ( \FILLnt{B} )^N   \FILLsym{)}      \FILLsym{)}     \FILLsym{,}   \lnot (  ( \Delta )^N  )   \FILLsym{,}   \lnot (  ( \Delta' )^N  )   \vdash   \cdot  }
      \end{math}
    \end{center}
    where
    \begin{center}
      \begin{math}
        \begin{array}{lll}
          D:\\
          \\
          $$\mprset{flushleft}
          \inferrule* [right=\ifrName{Impr}] {
            $$\mprset{flushleft}
            \inferrule* [right=\ifrName{Pr}] {
              $$\mprset{flushleft}
              \inferrule* [right=\ifrName{Parl}] {
                  \lnot (  \lnot (  ( \Gamma )^N  )  )   \FILLsym{,}  \FILLmv{x}  \FILLsym{:}   \lnot    \lnot  \FILLsym{(}   ( \FILLnt{A} )^N   \FILLsym{)}     \FILLsym{,}   \lnot (  ( \Delta )^N  )   \vdash   \cdot  
                \\
                  \lnot (  \lnot (  ( \Gamma' )^N  )  )   \FILLsym{,}  \FILLmv{v}  \FILLsym{:}   \lnot    \lnot  \FILLsym{(}   ( \FILLnt{B} )^N   \FILLsym{)}     \FILLsym{,}   \lnot (  ( \Delta' )^N  )   \vdash   \cdot  
              }{  \lnot (  \lnot (  ( \Gamma )^N  )  )   \FILLsym{,}   \lnot (  \lnot (  ( \Gamma' )^N  )  )   \FILLsym{,}  \FILLmv{y}  \FILLsym{:}     \lnot    \lnot  \FILLsym{(}   ( \FILLnt{A} )^N   \FILLsym{)}      \parr   \lnot    \lnot  \FILLsym{(}   ( \FILLnt{B} )^N   \FILLsym{)}      \FILLsym{,}   \lnot (  ( \Delta )^N  )   \FILLsym{,}   \lnot (  ( \Delta' )^N  )   \vdash   \cdot  }
            }{  \lnot (  \lnot (  ( \Gamma )^N  )  )   \FILLsym{,}   \lnot (  \lnot (  ( \Gamma' )^N  )  )   \FILLsym{,}  \FILLmv{y}  \FILLsym{:}     \lnot    \lnot  \FILLsym{(}   ( \FILLnt{A} )^N   \FILLsym{)}      \parr   \lnot    \lnot  \FILLsym{(}   ( \FILLnt{B} )^N   \FILLsym{)}      \FILLsym{,}   \lnot (  ( \Delta )^N  )   \FILLsym{,}   \lnot (  ( \Delta' )^N  )   \vdash   \circ   \FILLsym{:}   \perp  }
          }{  \lnot (  \lnot (  ( \Gamma )^N  )  )   \FILLsym{,}   \lnot (  \lnot (  ( \Gamma' )^N  )  )   \FILLsym{,}   \lnot (  ( \Delta )^N  )   \FILLsym{,}   \lnot (  ( \Delta' )^N  )   \vdash   \lambda  \FILLmv{y}  .   \circ    \FILLsym{:}   \lnot  \FILLsym{(}     \lnot    \lnot  \FILLsym{(}   ( \FILLnt{A} )^N   \FILLsym{)}      \parr   \lnot    \lnot  \FILLsym{(}   ( \FILLnt{B} )^N   \FILLsym{)}      \FILLsym{)}  }
        \end{array}
      \end{math}
    \end{center}
  \item[] Case.\\ 
    \begin{center}
      \begin{math}
        $$\mprset{flushleft}
        \inferrule* [right=\ifrName{Parr}] {
           \Gamma  \vdash    \Delta  \FILLsym{,}  \FILLnt{A}   \FILLsym{,}  \FILLnt{B}   \FILLsym{,}  \Delta' 
        }{ \Gamma  \vdash   \Delta  \FILLsym{,}   \FILLnt{A}  \parr  \FILLnt{B}    \FILLsym{,}  \Delta' }
      \end{math}
    \end{center}
    By the induction hypothesis we know the following is derivable:
    \[   \lnot (  \lnot (  ( \Gamma )^N  )  )   \FILLsym{,}   \lnot (  ( \Delta )^N  )   \FILLsym{,}  \FILLmv{x}  \FILLsym{:}   \lnot  \FILLsym{(}   ( \FILLnt{A} )^N   \FILLsym{)}   \FILLsym{,}  \FILLmv{y}  \FILLsym{:}   \lnot  \FILLsym{(}   ( \FILLnt{B} )^N   \FILLsym{)}   \FILLsym{,}   \lnot (  ( \Delta' )^N  )   \vdash   \cdot   \]
    It suffices to show that the sequent
    $ \lnot (  \lnot (  ( \Gamma )^N  )  )   \FILLsym{,}   \lnot (  ( \Delta )^N  )   \FILLsym{,}  \FILLmv{z}  \FILLsym{:}   \lnot  \FILLsym{(}   (  \FILLnt{A}  \parr  \FILLnt{B}  )^N   \FILLsym{)}   \FILLsym{,}   \lnot (  ( \Delta' )^N  ) $
    is derivable, but this sequent is equivalent to the sequent
    $ \lnot (  \lnot (  ( \Gamma )^N  )  )   \FILLsym{,}   \lnot (  ( \Delta )^N  )   \FILLsym{,}  \FILLmv{z}  \FILLsym{:}   \lnot  \FILLsym{(}     \lnot    \lnot  \FILLsym{(}   ( \FILLnt{A} )^N   \FILLsym{)}      \parr   \lnot    \lnot  \FILLsym{(}   ( \FILLnt{B} )^N   \FILLsym{)}      \FILLsym{)}   \FILLsym{,}   \lnot (  ( \Delta' )^N  ) $.
    We derive the latter as follows:
    \begin{center}
      \scriptsize
      \begin{math}
        $$\mprset{flushleft}
        \inferrule* [right=\ifrName{Impl}] {
          $$\mprset{flushleft}
          \inferrule* [right=\ifrName{Parr}] {
            $$\mprset{flushleft}
            \inferrule* [right=\ifrName{Impr}] {
              $$\mprset{flushleft}
              \inferrule* [right=\ifrName{Pr}] {
                $$\mprset{flushleft}
                \inferrule* [right=\ifrName{Impr}] {
                  $$\mprset{flushleft}
                  \inferrule* [right=\ifrName{Pr}] {
                      \lnot (  \lnot (  ( \Gamma )^N  )  )   \FILLsym{,}   \lnot (  ( \Delta )^N  )   \FILLsym{,}  \FILLmv{x}  \FILLsym{:}   \lnot  \FILLsym{(}   ( \FILLnt{A} )^N   \FILLsym{)}   \FILLsym{,}  \FILLmv{y}  \FILLsym{:}   \lnot  \FILLsym{(}   ( \FILLnt{B} )^N   \FILLsym{)}   \FILLsym{,}   \lnot (  ( \Delta' )^N  )   \vdash   \cdot  
                  }{  \lnot (  \lnot (  ( \Gamma )^N  )  )   \FILLsym{,}   \lnot (  ( \Delta )^N  )   \FILLsym{,}  \FILLmv{x}  \FILLsym{:}   \lnot  \FILLsym{(}   ( \FILLnt{A} )^N   \FILLsym{)}   \FILLsym{,}  \FILLmv{y}  \FILLsym{:}   \lnot  \FILLsym{(}   ( \FILLnt{B} )^N   \FILLsym{)}   \FILLsym{,}   \lnot (  ( \Delta' )^N  )   \vdash   \circ   \FILLsym{:}   \perp  }
                }{  \lnot (  \lnot (  ( \Gamma )^N  )  )   \FILLsym{,}   \lnot (  ( \Delta )^N  )   \FILLsym{,}  \FILLmv{x}  \FILLsym{:}   \lnot  \FILLsym{(}   ( \FILLnt{A} )^N   \FILLsym{)}   \FILLsym{,}   \lnot (  ( \Delta' )^N  )   \vdash   (  \lambda  \FILLmv{y}  .   \circ   )   \FILLsym{:}   \lnot    \lnot  \FILLsym{(}   ( \FILLnt{B} )^N   \FILLsym{)}    }
              }{  \lnot (  \lnot (  ( \Gamma )^N  )  )   \FILLsym{,}   \lnot (  ( \Delta )^N  )   \FILLsym{,}  \FILLmv{x}  \FILLsym{:}   \lnot  \FILLsym{(}   ( \FILLnt{A} )^N   \FILLsym{)}   \FILLsym{,}   \lnot (  ( \Delta' )^N  )   \vdash   \circ   \FILLsym{:}   \perp   \FILLsym{,}   (  \lambda  \FILLmv{y}  .   \circ   )   \FILLsym{:}   \lnot    \lnot  \FILLsym{(}   ( \FILLnt{B} )^N   \FILLsym{)}    }
            }{  \lnot (  \lnot (  ( \Gamma )^N  )  )   \FILLsym{,}   \lnot (  ( \Delta )^N  )   \FILLsym{,}   \lnot (  ( \Delta' )^N  )   \vdash   (  \lambda  \FILLmv{x}  .   \circ   )   \FILLsym{:}    \lnot    \lnot  \FILLsym{(}   ( \FILLnt{A} )^N   \FILLsym{)}      \FILLsym{,}   (  \lambda  \FILLmv{y}  .   \circ   )   \FILLsym{:}   \lnot    \lnot  \FILLsym{(}   ( \FILLnt{B} )^N   \FILLsym{)}    }
          }{  \lnot (  \lnot (  ( \Gamma )^N  )  )   \FILLsym{,}   \lnot (  ( \Delta )^N  )   \FILLsym{,}   \lnot (  ( \Delta' )^N  )   \vdash    (  \lambda  \FILLmv{x}  .   \circ   )   \parr   (  \lambda  \FILLmv{y}  .   \circ   )    \FILLsym{:}     \lnot    \lnot  \FILLsym{(}   ( \FILLnt{A} )^N   \FILLsym{)}      \parr   \lnot    \lnot  \FILLsym{(}   ( \FILLnt{B} )^N   \FILLsym{)}     }
          \\
            $$\mprset{flushleft}
          \inferrule* [right=\ifrName{Pl}] {
            \,
          }{ \FILLmv{w}  \FILLsym{:}   \perp   \vdash   \cdot  }
        }{ \lnot (  \lnot (  ( \Gamma )^N  )  )   \FILLsym{,}   \lnot (  ( \Delta )^N  )   \FILLsym{,}  \FILLmv{z}  \FILLsym{:}   \lnot  \FILLsym{(}     \lnot    \lnot  \FILLsym{(}   ( \FILLnt{A} )^N   \FILLsym{)}      \parr   \lnot    \lnot  \FILLsym{(}   ( \FILLnt{B} )^N   \FILLsym{)}      \FILLsym{)}   \FILLsym{,}   \lnot (  ( \Delta' )^N  ) }
      \end{math}
    \end{center}

  \item[] Case.\\
    \begin{center}
      \begin{math}
        $$\mprset{flushleft}
        \inferrule* [right=\ifrName{Negl}] {
           \Gamma  \FILLsym{,}  \FILLnt{A}  \vdash  \Delta 
        }{ \Gamma  \vdash   \FILLnt{A} ^{\perp}   \FILLsym{,}  \Delta }
      \end{math}
    \end{center}
    By the induction hypothesis we know the following:
    \[   \lnot (  \lnot (  ( \Gamma )^N  )  )   \FILLsym{,}  \FILLmv{x}  \FILLsym{:}   \lnot    \lnot  \FILLsym{(}   ( \FILLnt{A} )^N   \FILLsym{)}     \FILLsym{,}   \lnot (  ( \Delta )^N  )   \vdash   \cdot   \]
    It suffices to show that the sequent
    $  \lnot (  \lnot (  ( \Gamma )^N  )  )   \FILLsym{,}  \FILLmv{x}  \FILLsym{:}   \lnot  \FILLsym{(}   (  \FILLnt{A} ^{\perp}  )^N   \FILLsym{)}   \FILLsym{,}   \lnot (  ( \Delta )^N  )   \vdash   \cdot  $, but this is equivalent to the
    sequent
    $  \lnot (  \lnot (  ( \Gamma )^N  )  )   \FILLsym{,}  \FILLmv{x}  \FILLsym{:}   \lnot    \lnot  \FILLsym{(}   ( \FILLnt{A} )^N   \FILLsym{)}     \FILLsym{,}   \lnot (  ( \Delta )^N  )   \vdash   \cdot  $, but this is equivalent to the induction hypothesis.

    \item[] Case.\\
    \begin{center}
      \begin{math}
        $$\mprset{flushleft}
        \inferrule* [right=\ifrName{Negl}] {
           \Gamma  \vdash  \FILLnt{A}  \FILLsym{,}  \Delta 
        }{ \Gamma  \FILLsym{,}   \FILLnt{A} ^{\perp}   \vdash  \Delta }
      \end{math}
    \end{center}
    By the induction hypothesis we know the following:
    \[   \lnot (  \lnot (  ( \Gamma )^N  )  )   \FILLsym{,}  \FILLmv{x}  \FILLsym{:}   \lnot  \FILLsym{(}   ( \FILLnt{A} )^N   \FILLsym{)}   \FILLsym{,}   \lnot (  ( \Delta )^N  )   \vdash   \cdot   \]
    It suffices to show that the sequent
    $  \lnot (  \lnot (  ( \Gamma )^N  )  )   \FILLsym{,}  \FILLmv{z}  \FILLsym{:}   \lnot    \lnot  \FILLsym{(}   (  \FILLnt{A} ^{\perp}  )^N   \FILLsym{)}     \FILLsym{,}   \lnot (  ( \Delta )^N  )   \vdash   \cdot  $, but this is equivalent to the
    sequent
    $  \lnot (  \lnot (  ( \Gamma )^N  )  )   \FILLsym{,}  \FILLmv{z}  \FILLsym{:}   \lnot    \lnot  \FILLsym{(}   \lnot  \FILLsym{(}   ( \FILLnt{A} )^N   \FILLsym{)}   \FILLsym{)}     \FILLsym{,}   \lnot (  ( \Delta )^N  )   \vdash   \cdot  $.  The latter is derived as follows:
    \begin{center}
      \begin{math}
        $$\mprset{flushleft}
        \inferrule* [right=\ifrName{Impl}] {
          $$\mprset{flushleft}
          \inferrule* [right=\ifrName{Impr}] {
            $$\mprset{flushleft}
            \inferrule* [right=\ifrName{Pr}] {
                \lnot (  \lnot (  ( \Gamma )^N  )  )   \FILLsym{,}  \FILLmv{x}  \FILLsym{:}   \lnot  \FILLsym{(}   ( \FILLnt{A} )^N   \FILLsym{)}   \FILLsym{,}   \lnot (  ( \Delta )^N  )   \vdash   \cdot  
            }{  \lnot (  \lnot (  ( \Gamma )^N  )  )   \FILLsym{,}  \FILLmv{x}  \FILLsym{:}   \lnot  \FILLsym{(}   ( \FILLnt{A} )^N   \FILLsym{)}   \FILLsym{,}   \lnot (  ( \Delta )^N  )   \vdash   \circ   \FILLsym{:}   \perp  }
          }{  \lnot (  \lnot (  ( \Gamma )^N  )  )   \FILLsym{,}   \lnot (  ( \Delta )^N  )   \vdash   \lambda  \FILLmv{x}  .   \circ    \FILLsym{:}   \lnot  \FILLsym{(}   \lnot  \FILLsym{(}   ( \FILLnt{A} )^N   \FILLsym{)}   \FILLsym{)}  }
          \\
           \FILLmv{w}  \FILLsym{:}   \perp   \vdash   \cdot  
        }{  \lnot (  \lnot (  ( \Gamma )^N  )  )   \FILLsym{,}  \FILLmv{z}  \FILLsym{:}   \lnot    \lnot  \FILLsym{(}   \lnot  \FILLsym{(}   ( \FILLnt{A} )^N   \FILLsym{)}   \FILLsym{)}     \FILLsym{,}   \lnot (  ( \Delta )^N  )   \vdash   \cdot  }
      \end{math}
    \end{center}
    
  \item[] Case.\\ 
    \begin{center}
      \begin{math}
        $$\mprset{flushleft}
        \inferrule* [right=\ifrName{Exl}] {
           \Gamma  \FILLsym{,}  \FILLnt{A}  \FILLsym{,}  \FILLnt{B}  \vdash  \Delta 
        }{ \Gamma  \FILLsym{,}  \FILLnt{B}  \FILLsym{,}  \FILLnt{A}  \vdash  \Delta }
      \end{math}
    \end{center}
    This case follows by first applying the induction hypothesis and then applying
    the rule $\ifrName{Exl}$.

  \item[] Case.\\ 
    \begin{center}
      \begin{math}
        $$\mprset{flushleft}
        \inferrule* [right=\ifrName{Exr}] {
           \Gamma  \vdash    \Delta_{{\mathrm{1}}}  \FILLsym{,}  \FILLnt{A}   \FILLsym{,}  \FILLnt{B}   \FILLsym{,}  \Delta_{{\mathrm{2}}} 
        }{ \Gamma  \vdash    \Delta_{{\mathrm{1}}}  \FILLsym{,}  \FILLnt{B}   \FILLsym{,}  \FILLnt{A}   \FILLsym{,}  \Delta_{{\mathrm{2}}} }
      \end{math}
    \end{center}
    This case follows by first applying the induction hypothesis and then applying
    the rule $\ifrName{Exl}$.  
  \end{itemize}
  \end{report}
